Experiments/ProofChecking/PS.lean
@@ -1,0 +1,833 @@
+/-
+
+Persistent partial assignments and substitutions.
+
+Resizable arrays that can be ``cleared'' in O(1) time by bumping a generation
+number. Each cell in the array stores a generation number that determines if the
+cell is set (i.e. that it is above the data structure's generation number).
+Used to implement partial assignments and substitutions by assuming that all
+variables are unset (PPA) or set to themselves (PS) at initialization.
+
+Authors: Cayden Codel, Wojciech Nawrocki, James Gallicchio
+Carnegie Mellon University
+-/
+
+import LeanSAT.Data.Cnf
+import LeanSAT.Data.ICnf
+--import LeanSAT.AuxDefs
+import LeanSAT.Upstream.ToStd
+import LeanSAT.Upstream.ToMathlib
+import Mathlib.Data.Nat.Basic
+import LeanSAT.Model.Quantification
+import LeanSAT.Model.PropFun
+import LeanSAT.Data.PPA
+
+open LeanSAT LeanSAT.Model Nat
+open LitVar ILit IVar LawfulLitVar
+open PropFun
+
+/- The value contained in the partial substitution. Values can either be booleans
+   (in LRAT/LPR, they are only booleans), or set to other variables, with sign.
+
+  When set to other variables, the boolean indicates the sign (true is positive),
+  and the ILit refers to the underlying literal this variable is set to.     -/
+inductive PSVal where
+  | tr : PSVal
+  | fls : PSVal
+  | lit (l : ILit) : PSVal
+
+attribute [match_pattern] PSVal
+
+/- A PSCell is the actual array cell in the substitution. The generation
+   checks whether the cell is set (allowing for efficient clearing), and the val
+   field stores the information of what the variable is set to (boolean or other literal). -/
+structure PSCell where
+  generation : Nat   /- The generation value for the cell. Compare against PS.generation -/
+  val : PSVal
+
+/-- A persistent partial assignment of truth values to propositional variables.
+
+If used linearly, it is an efficient way of clearing out partial assignments
+when doing proof checking, tautology checking, or unit propagation. -/
+structure PS where
+  assignment : Array PSCell
+  /-- The generation counter is used to avoid clearing the assignment array.
+  Instead, we just bump the counter and interpret values in the array
+  below the counter as unassigned. -/
+  generation : PNat
+  /-- The maximum absolute value of any entry in `assignments`. -/
+  maxGen : Nat
+  le_maxGen : ∀ i ∈ assignment.data, i.generation ≤ maxGen
+
+/-! ## Reading values from the PS -/
+
+abbrev PSubst := (IVar → PropForm IVar)
+
+namespace PSVal
+
+@[simp, inline] def mkPosLit (idx : Nat) : PSVal := .lit (mkPos ⟨idx + 1, succ_pos _⟩)
+@[simp, inline] def mkNegLit (idx : Nat) : PSVal := .lit (mkNeg ⟨idx + 1, succ_pos _⟩)
+@[simp, inline] def mkFalse : PSVal := .fls
+
+protected def negate : PSVal → PSVal
+  | .tr => .fls
+  | .fls => .tr
+  | .lit l => .lit (LitVar.negate l)
+
+@[simp] theorem negate_negate : PSVal.negate ∘ PSVal.negate = id := by
+  ext r; cases r <;> simp [PSVal.negate]
+
+@[simp] theorem negate_negate' (r : PSVal) :
+    r.negate.negate = r := by
+  cases r <;> simp [PSVal.negate]
+
+theorem negate_rhs_eq_lhs_negate (r₁ r₂ : PSVal) :
+    r₁.negate = r₂ ↔ r₁ = r₂.negate := by
+  cases r₁ <;> cases r₂ <;> simp [PSVal.negate]; aesop
+
+@[simp] def isBool : PSVal →  Bool
+  | .tr => true
+  | .fls => true
+  | _ => false
+
+@[simp] def isLit : PSVal → Bool
+  | .lit _ => true
+  | _ => false
+
+@[simp] def getVar : PSVal → IVar
+  | .tr => 1  -- Useless return value for non-.lit values
+  | .fls => 1
+  | .lit l => toVar l
+
+@[simp] def getLit : PSVal → ILit
+  | .tr => mkPos ⟨1, succ_pos _⟩
+  | .fls => mkNeg ⟨1, succ_pos _⟩
+  | .lit l => l
+
+@[simp] def sign : PSVal → Bool
+  | .tr => true
+  | .fls => false
+  | .lit l => polarity l
+
+instance : ToString PSVal where
+  toString v :=
+    match v with
+    | .tr => "t"
+    | .fls => "f"
+    | .lit l => s!"{l}"
+
+end PSVal
+
+namespace PSCell
+
+/-
+def mkCell (idx : Nat) (gen : Nat := 0) : PSCell := {
+  generation := gen
+  val := PSVal.mkVal idx
+} -/
+
+def mkEmptyCell : PSCell := {
+  generation := 0
+  val := PSVal.mkFalse
+}
+
+-- Checks whether the cell is set against a provided generation value
+@[simp, inline] def isSet (c : PSCell) (gen : Nat) : Bool := (c.generation ≥ gen)
+@[simp, inline] def isBool (c : PSCell) : Bool := c.val.isBool
+@[simp, inline] def isLit (c : PSCell) : Bool := c.val.isLit
+@[simp, inline] def getVar (c : PSCell) : IVar := c.val.getVar
+@[simp, inline] def getLit (c : PSCell) : ILit := c.val.getLit
+@[simp, inline] def sign (c : PSCell) : Bool := c.val.sign
+@[simp, inline] def isPointer (c : PSCell) (gen : Nat) : Bool := c.isSet gen && c.isLit
+
+def varValue? (c : PSCell) (gen : Nat) : Option PSVal :=
+  if c.isSet gen then
+    some c.val
+  else
+    none
+
+@[simp, inline] def clear (c : PSCell) : PSCell := { c with generation := 0 }
+
+@[inline] def setToTrue (c : PSCell) (gen : Nat) : PSCell := { c with
+  generation := gen
+  val := PSVal.tr
+}
+
+@[inline] def setToFalse (c : PSCell) (gen : Nat) : PSCell := { c with
+  generation := gen
+  val := PSVal.fls
+}
+
+@[inline] def setToLit (c : PSCell) (l : ILit) (gen : Nat) : PSCell := { c with
+  generation := gen
+  val := PSVal.lit l
+}
+
+@[inline] def setLit (c : PSCell) (l : ILit) (gen : Nat) : PSCell :=
+  if polarity l then
+    c.setToTrue gen
+  else
+    c.setToFalse gen
+
+section /- generation -/
+
+variable (c : PSCell) (l : ILit) (gen : Nat)
+
+@[simp] theorem mkEmptyCell_generation : mkEmptyCell.generation = 0 := rfl
+@[simp] theorem setToTrue_generation : (c.setToTrue gen).generation = gen := rfl
+@[simp] theorem setToFalse_generation : (c.setToFalse gen).generation = gen := rfl
+@[simp] theorem setToLit_generation : (c.setToLit l gen).generation = gen := rfl
+@[simp] theorem setLit_generation : (c.setLit l gen).generation = gen := by
+  cases hpol : polarity l <;> simp [setLit, hpol]
+
+end /- generation -/
+
+instance : ToString PSCell where
+  toString c := s!"({c.generation}, {c.val})"
+
+end PSCell
+
+/-! # PS -/
+
+namespace PS
+
+@[inline] def size (τ : PS) : Nat := τ.assignment.size
+
+section /- Operations on Fin -/
+
+variable (τ : PS) (i : Fin τ.size)
+
+-- TODO: Or should these be abbrev?
+@[simp, inline] def get : PSCell := τ.assignment.get i
+@[simp, inline] def get? (i : Nat) : Option PSCell := τ.assignment.get? i
+
+@[simp, inline] def isSet : Bool := (τ.get i).isSet τ.generation
+@[simp, inline] def isLit : Bool := (τ.get i).isLit
+@[simp, inline] def getVar : IVar := (τ.get i).getVar
+@[simp, inline] def getLit : ILit := (τ.get i).getLit
+@[simp, inline] def sign : Bool := (τ.get i).sign
+@[simp, inline] def isPointer : Bool := (τ.get i).isPointer τ.generation
+
+end /- section -/
+
+section /- Operations on Nat -/
+
+variable (τ : PS) (i : Nat)
+
+-- TODO: Most elegant way to do Nats first? Monadic bind/map?
+@[simp, inline] def isSet? : Option Bool := (PSCell.isSet · τ.generation) <$> (τ.get? i)
+@[simp, inline] def isLit? : Option Bool := PSCell.isLit <$> (τ.get? i)
+@[simp, inline] def isPointer? : Option Bool := (PSCell.isPointer · τ.generation) <$> (τ.get? i)
+@[simp, inline] def getVar? : Option IVar := PSCell.getVar <$> (τ.get? i)
+@[simp, inline] def getLit? : Option ILit := PSCell.getLit <$> (τ.get? i)
+@[simp, inline] def sign? : Option Bool := PSCell.sign <$> (τ.get? i)
+
+end /- section -/
+
+instance : ToString PS where
+  toString τ := String.intercalate " ∧ "
+    (τ.assignment.foldl (init := []) (f := fun acc a => s!"{a}" :: acc))
+
+end PS
+
+/-! # WF: well-formed -/
+
+/-
+structure PSVal.WF (v : PSVal) (size : PNat) where
+  h_index : v.getLit.index < size
+
+structure PSCell.WF (c : PSCell) (size maxGen : PNat) where
+  h_val : PSVal.WF c.val size
+  h_gen : c.generation ≤ maxGen
+
+structure PS.WF (τ : PS) where
+  h_gen : τ.generation > 0
+  h_cells : ∀ (i : Fin τ.size), PSCell.WF (τ.get i)
+    ⟨τ.size, by match h : τ.size with
+                | 0     => rw [h] at i; exact Fin.elim0' i
+                | n + 1 => exact Nat.succ_pos _⟩ ⟨_, h_gen⟩ -/
+
+namespace PS
+
+/-! # varValue -/
+
+-- Cayden: @[simp] attribute here?
+def varValue (τ : PS) (v : IVar) : PSVal :=
+  if hi : v.index < τ.size then
+    match PSCell.varValue? (get τ ⟨v.index, hi⟩) τ.generation with
+    | none => PSVal.lit (mkPos v)
+    | some x => x
+  else
+    PSVal.lit (mkPos v)
+
+@[inline] def litValue (τ : PS) (l : ILit) : PSVal :=
+  if polarity l then
+    varValue τ (toVar l)
+  else
+    PSVal.negate (varValue τ (toVar l))
+
+def toSubst_fun (τ : PS) : PSubst → Fin τ.size → PSCell → PSubst :=
+  fun σ idx cell => (fun v =>
+    if v.index = idx.val then
+      match PSCell.varValue? cell v with
+      | none => σ v
+      | some .tr => PropForm.tr
+      | some .fls => PropForm.fls
+      | some (.lit l) => if polarity l then .var (toVar l)
+                         else .neg (.var (toVar l))
+    else σ v)
+
+def toSubst (τ : PS) : PSubst :=
+  τ.assignment.foldlIdx (init := .var) (toSubst_fun τ)
+
+theorem toSubst_fun_comm (τ : PS) :
+  ∀ (σ : PSubst) (idx₁ idx₂ : Fin τ.size),
+    (toSubst_fun τ) ((toSubst_fun τ) σ idx₁ (τ.get idx₁)) idx₂ (τ.get idx₂) =
+    (toSubst_fun τ) ((toSubst_fun τ) σ idx₂ (τ.get idx₂)) idx₁ (τ.get idx₁) := by
+  intro σ idx₁ idx₂
+  unfold toSubst_fun
+  apply funext
+  intro v
+  by_cases hidx : idx₁.val = idx₂.val
+  <;> by_cases hv₁ : v.index = idx₁.val
+  <;> by_cases hv₂ : v.index = idx₂.val
+  <;> try simp [hv₁, hv₂, hidx]
+  <;> try simp [hv₁, hv₂, hidx, Ne.symm hidx]
+
+theorem toSubst_of_comm (τ : PS) {v : IVar} (hv : v.index < τ.size) :
+    ∃ σ, τ.toSubst = (toSubst_fun τ) σ ⟨v.index, hv⟩ (τ.get ⟨v.index, hv⟩) :=
+  Array.foldlIdx_of_comm τ.assignment (toSubst_fun τ) .var (toSubst_fun_comm τ) ⟨v.index, hv⟩
+
+instance : ToString PS where
+  toString τ := String.intercalate " ∧ "
+    (τ.assignment.foldl (init := []) (f := fun acc a =>
+      match a.val with
+        | .tr => s!"{a.generation}" :: acc
+        | .fls => s!"-{a.generation}" :: acc
+        | .lit l => s!"<{l}>" :: acc))
+
+theorem litValue_negate (τ : PS) (l : ILit) :
+    (τ.litValue (-l)) = PSVal.negate (τ.litValue l) := by
+  cases hpol : polarity l <;> simp [hpol, litValue]
+
+theorem litValue_eq_varValue_pos {l : ILit} :
+    polarity l = true → ∀ (τ : PS), τ.litValue l = τ.varValue (toVar l) := by
+  intro hl; simp [hl, litValue]
+
+theorem litValue_eq_varValue_neg {l : ILit} :
+    polarity l = false → ∀ (τ : PS), τ.litValue l = PSVal.negate (τ.varValue (toVar l)) := by
+  intro hl; simp [hl, litValue]
+
+theorem lt_size_of_varValue_of_not_id {τ : PS} {v : IVar} :
+    τ.varValue v ≠ .lit (mkPos v) → v.index < τ.size := by
+  intro hv
+  by_contra
+  rename (¬v.index < τ.size) => h_con
+  simp [varValue, h_con] at hv
+
+theorem lt_size_of_litValue_of_not_id {τ : PS} {l : ILit} :
+    τ.litValue l ≠ .lit l → l.index < τ.size := by
+  intro hv
+  by_contra
+  rename (¬l.index < τ.size) => h_con
+  rcases mkPos_or_mkNeg l with (hl | hl)
+  -- Cayden TODO: put this in one simp [] call. Why explicit typeclass LawfulLitVar lemmas?
+  · simp [litValue, varValue, h_con] at hv
+    rw [hl] at hv
+    simp_rw [LawfulLitVar.polarity_mkPos, LawfulLitVar.toVar_mkPos] at hv
+    simp at hv
+  · simp [litValue, varValue, h_con, PSVal.negate] at hv
+    rw [hl] at hv
+    simp_rw [LawfulLitVar.polarity_mkNeg, LawfulLitVar.toVar_mkNeg] at hv
+    simp at hv
+
+theorem varValue_fls_iff {σ : PS} {v : IVar} :
+    (σ.varValue v = .fls) ↔ (PropFun.bind σ.toSubst ⟦v⟧) = ⊥ := by
+  sorry
+  done
+
+theorem varValue_tr_iff {σ : PS} {v : IVar} :
+    (σ.varValue v = .tr) ↔ (PropFun.bind σ.toSubst ⟦v⟧) = ⊤ := by
+  sorry
+  done
+
+theorem varValue_lit_iff {σ : PS} {v : IVar} {l : ILit} :
+    (σ.varValue v = .lit l) ↔ (PropFun.bind σ.toSubst ⟦v⟧) = (PropFun.bind σ.toSubst l) := by
+  sorry
+  done
+
+theorem litValue_fls_iff {σ : PS} {l : ILit} :
+    (σ.litValue l = .fls) ↔ (PropFun.bind σ.toSubst l) = ⊥ := by
+  sorry
+  done
+
+theorem litValue_tr_iff {σ : PS} {l : ILit} :
+    (σ.litValue l = .tr) ↔ (PropFun.bind σ.toSubst l) = ⊤ := by
+  sorry
+  done
+
+theorem litValue_lit_iff {σ : PS} {l₁ l₂ : ILit} :
+    (σ.litValue l₁ = .lit l₂) ↔ (PropFun.bind σ.toSubst l₁) = l₂ := by
+  sorry
+  done
+
+/-! # setLit -/
+
+-- Cayden TODO: How to make setF more efficient when the value needs to be a cell?
+-- Can an efficient implementation do this linearly? Ow will run out of memory?
+-- One idea is to use a .setF' that takes a function : (Option α → α) instead of value v : α
+-- That way, if the cell exists, its value can be mapped
+
+-- This is a more efficient version
+/-
+def setLit (τ : PS) (l : ILit) : PS := { τ with
+  assignment :=
+    if hidx : l.index < τ.size then
+      τ.assignment.set ⟨l.index, hidx⟩ ((τ.get ⟨l.index, hidx⟩).setLit l τ.generation)
+    else
+      τ.assignment.setF l.index (PSCell.mkEmptyCell.setLit l τ.generation) PSCell.mkEmptyCell
+  maxGen := max τ.maxGen τ.generation
+}
+-/
+
+theorem setVar_le_maxGen (τ : PS) (i : Nat) (c : PSCell) :
+    ∀ cell ∈ (τ.assignment.setF i c PSCell.mkEmptyCell).data, cell.generation ≤ max τ.maxGen c.generation := by
+  sorry
+  done
+
+-- This is a more functional version
+/-- Set the given literal to `true` for the current generation in the PS. -/
+def setLit (τ : PS) (l : ILit) : PS := { τ with
+  assignment := τ.assignment.setF l.index (PSCell.mkEmptyCell.setLit l τ.generation) PSCell.mkEmptyCell
+  maxGen := max τ.maxGen τ.generation
+  le_maxGen := by
+    have := setVar_le_maxGen τ l.index (PSCell.mkEmptyCell.setLit l τ.generation)
+    rwa [PSCell.setLit_generation PSCell.mkEmptyCell l ↑τ.generation] at this
+}
+
+/-- Set the given literal to `true` for all generations until `gen`. -/
+def setLitUntil (τ : PS) (l : ILit) (gen : Nat) : PS := { τ with
+  assignment := τ.assignment.setF l.index (PSCell.mkEmptyCell.setLit l gen) PSCell.mkEmptyCell
+  maxGen := max τ.maxGen gen
+  le_maxGen := by
+    have := setVar_le_maxGen τ l.index (PSCell.mkEmptyCell.setLit l gen)
+    rwa [PSCell.setLit_generation PSCell.mkEmptyCell l gen] at this
+}
+
+def setVarToLit (τ : PS) (v : IVar) (l : ILit) : PS := { τ with
+  assignment := τ.assignment.setF v.index (PSCell.mkEmptyCell.setLit l τ.generation) PSCell.mkEmptyCell
+  maxGen := max τ.maxGen τ.generation
+  le_maxGen := by
+    have := setVar_le_maxGen τ v.index (PSCell.mkEmptyCell.setLit l τ.generation)
+    rwa [PSCell.setLit_generation PSCell.mkEmptyCell l τ.generation] at this
+}
+
+def setVarToLitUntil (τ : PS) (v : IVar) (l : ILit) (gen : Nat) : PS := { τ with
+  assignment := τ.assignment.setF v.index (PSCell.mkEmptyCell.setLit l gen) PSCell.mkEmptyCell
+  maxGen := max τ.maxGen gen
+  le_maxGen := by
+    have := setVar_le_maxGen τ v.index (PSCell.mkEmptyCell.setLit l gen)
+    rwa [PSCell.setLit_generation PSCell.mkEmptyCell l gen] at this
+}
+
+@[simp, inline] def setLitToLit (τ : PS) (l l_target : ILit) : PS :=
+  if polarity l then
+    τ.setVarToLit (toVar l) l_target
+  else
+    τ.setVarToLit (toVar l) (-l_target)
+
+@[simp, inline] def setLitToLitUntil (τ : PS) (l l_target : ILit) (gen : Nat) : PS :=
+  if polarity l then
+    τ.setVarToLitUntil (toVar l) l_target gen
+  else
+    τ.setVarToLitUntil (toVar l) (-l_target) gen
+
+def setVars (σ : PS) (L : List (IVar × ILit)) : PS :=
+  L.foldl (init := σ) (fun σ ⟨v, l⟩ => σ.setVarToLit v l)
+
+def setVars' (σ : PS) (A : Array (IVar × ILit)) : PS :=
+  A.foldl (init := σ) (fun σ ⟨v, l⟩ => σ.setVarToLit v l)
+
+def setVarsUntil (σ : PS) (L : List (IVar × ILit)) (gen : Nat) : PS :=
+  L.foldl (init := σ) (fun σ ⟨v, l⟩ => σ.setVarToLitUntil v l gen)
+
+def setVarsUntil' (σ : PS) (A : Array (IVar × ILit)) (gen : Nat) : PS :=
+  A.foldl (init := σ) (fun σ ⟨v, l⟩ => σ.setVarToLitUntil v l gen)
+
+theorem setVars_eq_setVars' {L : List (IVar × ILit)} {A : Array (IVar × ILit)} :
+  L = A.data → ∀ (σ : PS), σ.setVars L = σ.setVars' A := by sorry
+
+/- Lemmas -/
+
+@[simp] theorem setLit_size (τ : PS) (l : ILit) : (τ.setLit l).size = max τ.size (l.index + 1) := by
+  simp [setLit, size]
+
+-- Cayden TODO: Figure out which things are @[simp] in def vs. @[simp] theorems.
+theorem litValue_setLit_pos (τ : PS) (l : ILit) : (τ.setLit l).litValue l = .tr := by
+  by_cases hpol : polarity l
+  <;> by_cases hl : l.index < τ.size
+  <;> simp [litValue, varValue, size, setLit, PSCell.setLit, PSCell.setToTrue, PSCell.setToFalse,
+        hpol, hl, PSCell.varValue?, PSVal.negate, Array.getElem_setF]
+
+theorem litValue_setLit_neg (τ : PS) {l₁ l₂ : ILit} :
+    l₁ ≠ l₂ → (τ.setLit l₁).litValue l₂ = τ.litValue l₂ := by
+  intro hne
+  by_cases hpol₁ : polarity l₁
+  · by_cases hpol₂ : polarity l₂
+    · simp [hpol₁, hpol₂, litValue]
+      sorry
+    sorry
+  /-by_cases hpol : polarity l₂
+  · simp [litValue, hpol, setLit, Array.size_setF, -Array.get_eq_getElem]
+    by_cases hl₂ : l₂.index < τ.size
+    · rw [size] at hl₂
+      have : l₂.index < τ.assignment.size ∨ l₂.index < l₁.index + 1 := Or.inl hl₂
+      simp [hl₂, this, -Array.get_eq_getElem]
+      by_cases hpol₁ : polarity l₁
+      · rw [Array.getElem_setF' τ.assignment l₁.index ⟨τ.generation, PSVal.tr⟩ PSCell.mkEmptyCell]
+
+      done
+    done
+  --by_cases hpol : polarity l₂
+  --<;> by_cases hl₂ : l₂.index < τ.size
+  --<;> simp [litValue, setLit, hpol,
+  --    hl₂, Or.inl hl₂, Array.size_setF, PSCell.varValue?, PSVal.negate] -/
+  sorry
+  done
+
+/-! # New -/
+
+--ofFn (fun (idx : Fin maxVar) => PSCell.mkCell idx 0)
+
+/-- Initialize to an empty partial assignment,
+supporting variables in the range `[1, maxVar]`.
+
+The assignment will resize dynamically if it's used with
+a variable above the initial `maxVar`. -/
+
+def new (n : Nat) : PS where
+  assignment := Array.mkArray n PSCell.mkEmptyCell
+  generation := ⟨1, Nat.one_pos⟩
+  maxGen := 0
+  le_maxGen := by simp_all [List.mem_replicate]
+
+/-
+theorem new_WF (n : Nat) : (new n).WF := by
+  simp [new]
+  constructor
+  · intro i
+    sorry
+  · simp only [gt_iff_lt, zero_lt_one] -/
+
+/-! # Reset -/
+
+/-- Reset the assignment to an empty one. -/
+def reset (τ : PS) : PS :=
+  { τ with
+    generation := ⟨τ.maxGen + 1, Nat.succ_pos _⟩ }
+
+/-! # Bump -/
+
+/-- Clear all temporary assignments at the current generation. -/
+def bump (τ : PS) : PS :=
+  { τ with generation := τ.generation + 1 }
+
+
+section monadic
+
+/-! # Unit propagation -/
+
+/-
+
+Cayden note 1/8: In SR checking, the substitution witness σ is provided in the proof line,
+  and then never modified. Instead, a partial assignment α is produced and modified.
+
+To save memory and time, the substitution and partial assignments use the "generation bumping" strategy
+to clear out their computations after each proof line/group of hints.
+
+Since unit propagation is never done/evaluated against a substitution, proving its correctness is moot.
+But! We do need to compute a clause's reduction under a substitution, and so we need a theory for that.
+We also need to think about an efficient way to either compute a reduction OR make reduction and evaluation
+against a partial assignment happen in the same step (possibly using another "PPA" structure off to the side
+to record which literals have been seen in the reduction, so a tautology can be detected)
+
+-/
+
+inductive UPResult where
+  | falsified
+  | satisfied
+  | unit (l : ILit) (τ : PS) -- Updated substitution and unit literal l
+  | multipleUnassignedLiterals
+
+inductive UPDone where
+  | satisfied
+  | multipleUnassignedLiterals
+
+abbrev UPBox := ResultT UPDone (Option ILit)
+
+open ResultT UPResult UPDone PPA
+
+def sevalUP (σ : PS) (unit? : Option ILit) (l : ILit) : UPBox :=
+  match σ.litValue l with
+  | .tr => done .satisfied
+  | .fls => ok unit?
+  | .lit lit =>
+    match unit? with
+    | none => ok lit
+    | some u =>
+      if u = lit then ok unit?
+      -- Since σ is a substitution, tautology could occur
+      else if u = -lit then done .satisfied
+      else done .multipleUnassignedLiterals
+
+def foldUP (σ : PS) (C : IClause) := C.foldlM (sevalUP σ) none
+
+def unitProp (σ : PS) (C : IClause) : UPResult :=
+  match foldUP σ C with
+  | ok none => .falsified
+  | ok (some lit) => .unit lit (σ.setLit lit)
+  | done .satisfied => .satisfied
+  | done .multipleUnassignedLiterals => .multipleUnassignedLiterals
+
+def UP_motive_fn (σ : PS) (C : IClause) : ℕ → Option ILit → Prop
+  | idx, none => ∀ ⦃i : Fin C.size⦄, i < idx → σ.litValue C[i] = .fls
+  | idx, some lit => ∃ (i : Fin C.size), i < idx ∧ σ.litValue C[i] = .lit lit ∧
+      (∀ ⦃j : Fin C.size⦄, j < idx → j ≠ i → (σ.litValue C[j] = .fls ∨ σ.litValue C[j] = .lit lit))
+
+theorem SatisfiesM_UP (σ : PS) (C : IClause) :
+    SatisfiesM (fun
+      | none => ∀ l ∈ C.data, σ.litValue l = .fls
+      | some lit => ∃ (l : ILit), l ∈ C.data ∧ σ.litValue l = .lit lit ∧
+          (∀ l' ∈ C.data, l' ≠ l → (σ.litValue l' = .fls ∨ σ.litValue l' = .lit lit))) (foldUP σ C) := by
+  have := C.SatisfiesM_foldlM (init := (none : Option ILit)) (f := sevalUP σ)
+    (motive := UP_motive_fn σ C)
+    (h0 := by simp [UP_motive_fn])
+    (hf := by
+      unfold UP_motive_fn
+      simp only [SatisfiesM_ResultT_eq, getElem_fin]
+      -- Cayden question: is the proof more compact if I use pattern-matching with intro?
+      intro i box ih
+      intro
+      | none, hbox =>
+        intro j hj
+        unfold sevalUP at hbox
+        match hσ : σ.litValue C[i.val] with
+        | .tr => simp_rw [hσ] at hbox
+        | .fls =>
+          simp_rw [hσ, ok.injEq] at hbox; subst hbox
+          rcases Order.lt_succ_iff_eq_or_lt.mp hj with (hj | hj)
+          · rw [Fin.ext hj]; exact hσ
+          · exact ih hj
+        | .lit lit =>
+          simp [hσ] at hbox
+          match box with
+          | none => simp at hbox
+          | some u =>
+            rcases eq_trichotomy u lit with (rfl | rfl | hvar)
+            · simp at hbox
+            · simp at hbox
+            · simp [ne_of_var_ne hvar, ne_of_var_ne ((toVar_negate lit).symm ▸ hvar)] at hbox
+      | some u, hbox =>
+        rename ILit => lit
+        unfold sevalUP at hbox
+        match hσ : σ.litValue C[i.val] with
+        | .tr => simp_rw [hσ] at hbox
+        | .fls =>
+          simp_rw [hσ, ok.injEq] at hbox; subst hbox
+          rcases ih with ⟨idx, hidx_lt, hidxσ, hidx_fls⟩
+          use idx, lt_succ_of_lt hidx_lt, hidxσ
+          intro j hj
+          rcases lt_or_eq_of_le (le_of_lt_succ hj) with (h | h)
+          · exact hidx_fls h
+          · replace h := Fin.ext h; subst h; intro _; exact Or.inl hσ
+        | .lit lit' =>
+          simp [hσ] at hbox
+          match box with
+          | none =>
+            simp at hbox; subst hbox
+            have : C[i.val] ∈ C.data := Array.getElem_mem_data C i.isLt
+            use i, lt_succ_self _, hσ
+            intro j hj
+            rcases lt_or_eq_of_le (le_of_lt_succ hj) with (h | h)
+            · intro _; exact Or.inl (ih h)
+            · replace h := Fin.ext h; subst h; intro hcon; contradiction
+          | some u =>
+            rcases eq_trichotomy u lit' with (rfl | rfl | hvar)
+            · simp at hbox; subst hbox
+              rcases ih with ⟨idx, hidx_lt, hidxσ, hidx_fls⟩
+              use idx, lt_succ_of_lt hidx_lt, hidxσ
+              intro j hj
+              rcases lt_or_eq_of_le (le_of_lt_succ hj) with (h | h)
+              · exact hidx_fls h
+              · replace h := Fin.ext h; subst h; intro _; exact Or.inr hσ
+            · simp at hbox
+            · simp [ne_of_var_ne hvar, ne_of_var_ne ((toVar_negate lit').symm ▸ hvar)] at hbox)
+  apply SatisfiesM.imp this
+  intro
+  | none =>
+    intro h l hl
+    rcases Array.mem_data_iff.mp hl with ⟨i, rfl⟩
+    exact h i.isLt
+  | some lit =>
+    simp [UP_motive_fn]
+    intro i hi ih
+    use C[i.val], Array.getElem_mem_data C i.isLt, hi
+    intro l hl₁ hl₂
+    rcases Array.mem_data_iff.mp hl₁ with ⟨j, rfl⟩
+    apply ih
+    exact ne_of_apply_ne (C[·]) hl₂
+
+theorem contradiction_of_UP_falsified {σ : PS} {C : IClause} :
+    σ.unitProp C = .falsified → (C.toPropFun).bind σ.toSubst ≤ ⊥ := by
+  unfold unitProp
+  intro h_falsified
+  split at h_falsified <;> try simp at h_falsified
+  clear h_falsified
+  rename (foldUP σ C = ok none) => h
+  refine entails_ext.mpr fun τ hτ => ?_
+  rw [satisfies_bind] at hτ
+  have ⟨lit, hlit, hτlit⟩ := Clause.satisfies_iff.mp hτ
+  have := SatisfiesM_ResultT_eq.mp (SatisfiesM_UP σ C) none h lit hlit
+  clear h hτ
+  replace hτlit := satisfies_iff.mp hτlit
+  cases hpol : polarity lit
+  <;> simp [hpol, PropAssignment.preimage] at hτlit
+  · rw [litValue_eq_varValue_neg hpol, PSVal.negate_rhs_eq_lhs_negate, PSVal.negate,
+          varValue_tr_iff, bind_distrib] at this
+    rw [this] at hτlit
+    contradiction
+  · rw [litValue_eq_varValue_pos hpol, varValue_fls_iff, bind_distrib] at this
+    rw [this] at hτlit
+    exact hτlit
+
+theorem extended_of_UP_unit {σ σ' : PS} {C : IClause} {l : ILit} :
+    σ.unitProp C = .unit l σ' →
+      (C.toPropFun).bind σ.toSubst ≤ l.toPropFun ∧
+      (∃ lit ∈ C.data, σ.litValue lit = .lit l ∧ σ'.litValue l = .tr) := by
+      -- Cayden question: how to express this in an abstract way? Perhaps with a bind (l.bind σ) or as a (. ∘ .) of two subs
+  unfold unitProp
+  intro h_unit
+  split at h_unit <;> try simp at h_unit
+  --clear h_unit
+  rename ILit => lit
+  rename (foldUP σ C = ok (some lit)) => h
+  rcases h_unit with ⟨rfl, rfl⟩
+  have hlv := SatisfiesM_ResultT_eq.mp (SatisfiesM_UP σ C) (some lit) h
+  clear h
+  rcases hlv with ⟨l, hl_mem, hσl, ih⟩
+  constructor
+  · refine entails_ext.mpr fun τ hτ => ?_
+    rw [satisfies_bind] at hτ
+    by_cases heq : l = lit
+    · subst heq
+      rw [Clause.satisfies_iff] at hτ; rcases hτ with ⟨l', hl'_mem, hl'⟩
+      rw [← satisfies_bind] at hl'
+      sorry -- Proof got stuck here. And we may not need unit propagaion after all
+      done
+    · sorry
+      done
+    done
+  · exact ⟨l, hl_mem, hσl, litValue_setLit_pos _ _⟩
+  done
+
+-- We have to carry along a PPA to store the unset literals and check for tautologies (Cayden later comment: why??)
+
+/-! # Reduction -/
+
+-- We do something very similar to "unit propagation", except we don't modify σ
+
+inductive ReductionResult where
+  | falsified
+  | satisfied
+  | reduced
+  | notReduced
+
+abbrev RedBox := ResultT PPA (PPA × Bool × Bool)
+
+open ResultT ReductionResult
+
+def sevalRed (σ : PS) (p : PPA × Bool × Bool) (l : ILit) : RedBox :=
+  let ⟨τ, reduced?, unassigned?⟩ := p
+  match σ.litValue l with
+  | .tr => done τ
+  | .fls => ok ⟨τ, true, unassigned?⟩
+  | .lit lit =>
+    match τ.litValue? lit with
+    | none => ok ⟨τ.setLit lit, reduced? || (l != lit), true⟩
+    | some true => ok ⟨τ, reduced? || (l != lit), true⟩
+    | some false => done τ
+
+def foldRed (σ : PS) (τ : PPA) (C : IClause) := C.foldlM (sevalRed σ) ⟨τ.reset, false, false⟩
+
+def reduced? (σ : PS) (τ : PPA) (C : IClause) : ReductionResult × PPA :=
+  match foldRed σ τ C with
+  | ok ⟨τ, true, false⟩  => (.falsified, τ)
+  | ok ⟨τ, true, true⟩   => (.reduced, τ)
+  | ok ⟨τ, false, true⟩  => (.notReduced, τ)
+  | ok ⟨τ, false, false⟩ => (.notReduced, τ) -- Shouldn't get this case, except if C is empty
+  | done τ => (.satisfied, τ)
+
+theorem reduced?_satisfied_iff {σ : PS} {τ τ' : PPA} {C : IClause} :
+    σ.reduced? τ C = (.satisfied, τ') ↔ (C.toPropFun).bind σ.toSubst = ⊤ := by
+  sorry
+  done
+
+theorem reduced?_falsified_iff {σ : PS} {τ τ' : PPA} {C : IClause} :
+    σ.reduced? τ C = (.falsified, τ') ↔ (C.toPropFun).bind σ.toSubst ≤ ⊥ := by
+  sorry
+  done
+
+theorem reduced?_notReduced_iff {σ : PS} {τ τ' : PPA} {C : IClause} :
+    σ.reduced? τ C = (.notReduced, τ') ↔ (C.toPropFun).bind σ.toSubst = ↑C := by
+  sorry
+  done
+
+theorem reduced?_reduced {σ : PS} {τ τ' : PPA} {C : IClause} :
+    σ.reduced? τ C = (.reduced, τ') →
+      ((C.toPropFun).bind σ.toSubst ≠ ⊤ ∧ (C.toPropFun).bind σ.toSubst ≠ ⊥) := by
+  sorry
+  done
+
+/- Reduction without tautology checking -/
+
+def seval (σ : PS) (p : Bool × Bool) (l : ILit) : ResultT Unit (Bool × Bool) :=
+  -- Has there been a non-id map, and has there been an literal that's unassigned
+  let ⟨reduced?, unassigned?⟩ := p
+  match σ.litValue l with
+  | .tr => done ()
+  | .fls => ok (true, unassigned?)
+  | .lit lit => ok (reduced? || (l != lit), true)
+
+def reduce (σ : PS) (C : IClause) : ReductionResult :=
+  match C.foldlM (seval σ) (false, false) with
+  | ok (true, true) => .reduced
+  | ok (true, false) => .falsified
+  | ok (false, true) => .notReduced
+  | ok (false, false) => .notReduced -- Shouldn't get this, unless if C is empty
+  | done () => .satisfied
+
+-- TODO: It is possible only the forward directions are needed
+theorem reduce_satisfied_iff {σ : PS} {C : IClause} :
+    σ.reduce C = .satisfied ↔ (C.toPropFun).bind σ.toSubst = ⊤ := by
+  sorry
+  done
+
+theorem reduce_falsified_iff {σ : PS} {C : IClause} :
+    σ.reduce C = .falsified ↔ (C.toPropFun).bind σ.toSubst ≤ ⊥ := by
+  sorry
+  done
+
+theorem reduce_notReduced_iff {σ : PS} {C : IClause} :
+    σ.reduce C = .notReduced ↔ (C.toPropFun).bind σ.toSubst = ↑C := by
+  sorry
+  done
+
+theorem reduce_reduced {σ : PS} {C : IClause} :
+    σ.reduce C = .reduced ↔
+      ((C.toPropFun).bind σ.toSubst ≠ ⊤ ∧ (C.toPropFun).bind σ.toSubst ≠ ⊥) := by
+  sorry
+  done
+
+end monadic
+
+end PS
